proof/old_system/uni/def_ott.v
@@ -1452,7 +1452,10 @@ Inductive d_sub : denv -> typ -> typ -> Prop :=    (* defn d_sub *)
  | d_sub__union3 : forall (Ψ:denv) (A1 A2 B:typ),
      d_sub Ψ A1 B ->
      d_sub Ψ A2 B ->
-     d_sub Ψ (typ_union A1 A2) B.
+     d_sub Ψ (typ_union A1 A2) B
+ | d_sub__all_refl : forall (L:vars) (Ψ:denv) (A1:typ),
+      ( forall X , X \notin  L  -> d_sub Ψ  ( open_typ_wrt_typ A1 (typ_var_f X) )   ( open_typ_wrt_typ A1 (typ_var_f X) )  )  ->
+     d_sub Ψ (typ_all A1) (typ_all A1).
 
 (* defns J_a_wf_typ *)
 Inductive a_wf_typ : aenv -> typ -> Prop :=    (* defn a_wf_typ *)
